\documentclass{report}

\usepackage{amsmath}
\usepackage[thinc]{esdiff}

\title{Project Report — Ice-Ocean Interaction}
\author{David Sermoneta, Emma Bastås}

\begin{document}

\maketitle

The given equation:

\begin{gather*}
  \diffp{C}{t} = \nu \diffp{C}{{x^2}} - \diffp{u(x)C}{x} = 0 \\
  \diffp{C}{t} = 0 \quad \text{(We are in steady-state)} \\
\end{gather*}

Simplification:

\begin{gather}
  \nu y'' - u'y - uy' = 0 \label{eq}\tag{$\star$}\text{.}
\end{gather}

We use centered difference to approximate $y'$ and $y''$:

\begin{gather*}
  y_i' = \frac{y_{i+1} - y_{i-1}}{2h} \\[3pt]
  y_i'' = \frac{y_{i+1} - 2y_i + y_{i-1}}{h^2}
\end{gather*}

Thus:

\begin{gather*}
  \text{(\ref{eq})} \implies
  \nu\frac{y_{i+1} - 2y_i + y_{i-1}}{h^2}
  - u_i'y
  -u_i\frac{y_{i+1} - y_{i-1}}{2h} = \\
  \biggl(\frac{\nu}{h^2} + \frac{u_i}{2h}\biggr)y_{i-1} - \biggl(\frac{2\nu}{h^2} + u_i'\biggr) + \biggl(\frac{\nu}{h^2} - \frac{u_i}{2h}\biggr)y_{i+1} = 0
\end{gather*}


\end{document}
